Arithmetic: more general partial order with isomorphic addresses

Arithmetic/theories/Environnement.v
@@ -1,6 +1,6 @@
 From RAC Require Import Utils.
 From RAC.Languages Require Import Syntax.
-From Coq Require Import ZArith.ZArith Strings.String.
+From Coq Require Import ZArith.ZArith Strings.String Logic.FinFun.
 From RecordUpdate Require Import RecordUpdate.
 
 
@@ -33,8 +33,13 @@ Definition zero :=  0ⁱⁿᵗ zeroinRange.
 Definition one := 1ⁱⁿᵗ oneinRange.
 Definition sub_one := (-1)ⁱⁿᵗ suboneinRange.
 
+
+
+(* adresses and undefined values must be an enumerable set. We use nat for convenience *)
 Definition location := nat. 
-#[global] Instance location_eq_dec : EqDec location := {eq_dec := Nat.eq_dec}.
+Definition undefval := nat.
+
+#[global] Instance location_eq_dec : EqDecC location := {eq_dec := Nat.eq_dec}.
 
 
 
@@ -49,27 +54,33 @@ Inductive value :=
     | VMpz (l:option location) (* memory location for values of type mpz, none is a null pointer *) 
 .
 
+
 Inductive undef := 
-    | UInt (n:Int.MI) (* set of undefined values of type int *) 
-    | UMpz (l:option location) (* set of undefined values of type mpz *) 
+    | UInt : undefval -> undef (* set of undefined values of type int *) 
+    | UMpz : undefval -> undef (* set of undefined values of type mpz *) 
 .
 
+
 Inductive 𝕍 :=  Def (v : value) :> 𝕍 | Undef (uv : undef) :> 𝕍.
+Coercion v_int (mi:Int.MI) : 𝕍 := Def (VInt mi). 
+Coercion def_v_mpz (l:nat) : 𝕍 := Def (VMpz (Some l)). 
+Coercion mpz_loc (l:location) : 𝕍 := VMpz (Some l).
 
 Inductive 𝔹 := BTrue | BFalse.
 
 Inductive mpz_val := Defined (z:Z) :> mpz_val | Undefined (z:Z).
 
+
 Definition 𝓜 := location ⇀ mpz_val. 
+
+
 Definition Ωᵥ : Type := 𝓥 ⇀ 𝕍.
 Definition Ωₗ : Type := 𝔏 ⇀ ℤ.
 
 
 (* Coercion ir_z (x:Z) ir : 𝕍 := VInt (x ⁱⁿᵗ ir). *)
 Coercion int_option_loc (l:nat) :=  Some l.
-Coercion v_int (mi:Int.MI) : 𝕍 := Def (VInt mi). 
-Coercion def_v_mpz (l:nat) : 𝕍 := Def (VMpz (Some l)). 
-Coercion mpz_loc (l:location) : 𝕍 := VMpz (Some l).
+
 
 (* Coercion VMpz : nat >-> Value. *)
 (* 
@@ -97,22 +108,57 @@ Definition apply_mem (a : Ω) (l : 𝔏) : option Z := a.(binds) l.
 (* Coercion apply_mem : Ω >-> Funclass. *) (* can't use same coercion path *)
 
 
-Inductive param_env_partial_order (var: 𝓥) (env env':Ω) : Prop :=
+Definition σ : Type := {f : location -> location | Bijective f}.
+
+Fact bijective_eq_iff_f_eq  {A B:Type} : forall (f: A -> B) x y , Bijective f -> x = y <-> f x = f y. 
+Proof.
+    intros. destruct H as [f_inv [H1 H2]]. split ; congruence.
+Qed.
+
+
+Definition induced (f: σ) : 𝕍 -> 𝕍 := fun value => match value with
+| Def (VMpz (Some l)) => Def (VMpz (Some (proj1_sig f l)))
+| v => v
+end.
+
+Fact induced_not_mpz_transparent (f: σ) : forall v, 
+    (forall l, v <> Def (VMpz (Some l))) -> induced f v = v.
+Proof.
+        intros. destruct v; auto. destruct v; auto. destruct l; auto. congruence.
+Qed.
+
+Fact induced_int_iff (f: σ) : forall v n, 
+    induced f v = (VInt n) <-> v = VInt n.
+Proof.
+        intros. split; intros H.
+        - unfold induced in H. simpl in H. destruct v; try congruence.
+            destruct v; try congruence. now destruct l.
+        - subst. now apply induced_not_mpz_transparent.
+Qed.
+
+
+Inductive param_env_partial_order (env env':Ω) (var: 𝓥) (f:σ) : Prop :=
 | EsameInt n : 
     env var = Some (Def (VInt n))
     ->  env' var = Some (Def (VInt n))
-    -> param_env_partial_order var env env'
-| EsameMpz l : 
-    env var = Some (Def (VMpz l))
-    -> env' var = Some (Def (VMpz l))
-    -> param_env_partial_order var env env'
-| EundefInt n: env var = Some (Undef (UInt n))
-    -> env' var = Some (Undef (UInt n)) \/  (exists n, env' var = Some (Def (VInt n)))
-    -> param_env_partial_order var env env'
-| EundefMpz n : env var = Some (Undef (UMpz n))
-    -> env' var = Some (Undef (UMpz n)) \/  (exists n, env' var = Some (Def (VMpz n)))
-    -> param_env_partial_order var env env'
-| Enone : env var = None -> param_env_partial_order var env env'
+    -> param_env_partial_order env env' var f
+| EsameMpz (l:location) : 
+    (* if the mpz is not a null pointer, we must have a corresponding adress *)
+    env var = Some (Def (VMpz l)) ->
+    env' var = Some (Def (VMpz (proj1_sig f l)))
+    -> param_env_partial_order env env' var f
+| ENullPtr : 
+    (* if the mpz is a null pointer, it must stay null *)
+    env var = Some (Def (VMpz None)) ->
+    env' var = Some (Def (VMpz None))
+    -> param_env_partial_order env env' var f
+| EundefInt u : env var = Some (Undef (UInt u))
+    -> (exists u', env' var = Some (Undef (UInt u'))) \/  (exists n, env' var = Some (Def (VInt n)))
+    -> param_env_partial_order env env' var f
+| EundefMpz u: env var = Some (Undef (UMpz u))
+    -> (exists u, env' var = Some (Undef (UMpz u))) \/  (exists l, env' var = Some (Def (VMpz l)))
+    -> param_env_partial_order env env' var f
+| Enone : env var = None -> param_env_partial_order env env' var f
 .
 
 #[global] Hint Constructors param_env_partial_order : rac_hint.
@@ -124,74 +170,140 @@ Delimit Scope mem_scope with mem.
 Declare Scope env_mem_scope.
 Delimit Scope env_mem_scope with envmem.
 
-Definition env_partial_order env env' := forall v, param_env_partial_order v env env'.
-Infix "⊑" := env_partial_order : env_scope.
+Definition existify {A} (p: A -> Prop) : Prop := exists a, p a. 
 
-Definition mems_partial_order (mem mem':𝓜) : Prop := forall l i, mem l = Some i ->  mem' l = Some i.
-Infix "⊑" := mems_partial_order : mem_scope.
+Definition env_partial_order env env' := fun f => forall v, param_env_partial_order env env' v f.
+Infix "⊑" := (fun e e' =>  existify (env_partial_order e e') ) : env_scope.
 
 
-Infix "⊑" :=  ( fun e e' => (e.(env) ⊑ e'.(env))%env /\ (e.(mstate) ⊑ e'.(mstate))%mem) : env_mem_scope.
+Definition param_mem_partial_order (mem mem':𝓜)  (l: location) (f:σ) := forall i, mem l = Some i ->  (mem' (proj1_sig f l)) = Some i.
+Definition mem_partial_order env env' := fun f => forall l, param_mem_partial_order env env' l f.
+Infix "⊑" := (fun e e' =>  existify (mem_partial_order e e') ) : mem_scope.
+
+
+Definition env_mem_partial_order e e' f := 
+    env_partial_order e.(env) e'.(env) f /\ mem_partial_order e.(mstate) e'.(mstate) f.
+Infix "⊑" := (fun e e' =>  existify (env_mem_partial_order e e') ) : env_mem_scope.
+
+
+Open Scope utils_scope.
+
+
+Fact id_bijective {T:Type} : @Bijective T T (fun T => T). 
+Proof.
+    now exists (fun x => x).
+Qed.
+
+Fact bijective_comp_bijective {A B C: Type} (fa: {f: A -> B | Bijective f}) (fb: {f: B -> C | Bijective f}) : 
+    Bijective (fun x => (proj1_sig fb) (proj1_sig fa x)).
+Proof. 
+    destruct fa as [a [a_inv [a1 a2]]] ,fb as [b [b_inv [b1 b2]]].
+    exists (fun x => a_inv (b_inv x)). simpl in *. split ; congruence. 
+Qed.
 
 
 (* Environnement Properties *)
 From Coq Require Import Setoid.
-Fact refl_env_partial_order : reflexive Ω env_partial_order.
+
+Fact _refl_env_partial_order : reflexive Ω (fun e e' => env_partial_order e e' (exist _ _ id_bijective)).
+
 Proof.
     intros [v l] var. destruct (v var) as [val |] eqn:res. induction val.
     - destruct v0.
         * now apply EsameInt with n.
-        * now apply EsameMpz with l0. 
+        * destruct l0 as [l0|].
+            ** now apply EsameMpz with l0. 
+            ** now apply ENullPtr.
     - destruct uv.
-        * apply EundefInt with n; auto.
-        * apply EundefMpz with l0; auto.
+        * apply EundefInt with u; eauto.
+        * apply EundefMpz with u; eauto.
     - apply Enone ; auto.
 Qed.
 
+Corollary refl_env_partial_order :  reflexive Ω (fun e e' => e ⊑ e')%env.
+Proof. 
+    eexists. apply _refl_env_partial_order.
+Qed.
 
-Fact trans_env_partial_order : transitive Ω env_partial_order.
+Fact _trans_env_partial_order : forall (x y z:Ω) f1 f2, 
+    env_partial_order x y f1 ->
+    env_partial_order y z f2 -> 
+    env_partial_order x z (exist _ _ (bijective_comp_bijective f1 f2)).
 Proof.
-    intros  [v l] [v' l'] [v'' l'']  H1 H2 var. destruct H1 with var ; specialize (H2 var).
-    * apply EsameInt with n. easy. inversion H2 ; congruence.
-    * apply EsameMpz with l0 ; inversion H2; congruence.
-    * apply EundefInt with n.
+    intros  e e' e''  sub1 sub2 Hrel1 Hrel2 var. destruct Hrel1 with var ; specialize (Hrel2 var).
+    * apply EsameInt with n. easy. inversion Hrel2 ; congruence.
+    * apply EsameMpz with l ; inversion Hrel2; simpl in * ; try congruence.
+        ** rewrite H0 in H1. inversion H1. now subst.
+        ** now rewrite H1 in H0. 
+    * apply ENullPtr;[easy|]. inversion Hrel2; simpl in *; try congruence. now  rewrite H0 in H1.
+    * apply EundefInt with u.
         + assumption.
-        + inversion H2 ; destruct H0 ; eauto ; try congruence ; try (destruct H0 ; congruence).
-    * apply EundefMpz with n. easy. inversion H2; destruct H0; try congruence || (destruct H0 ; congruence). right. now exists l0.
+        + inversion Hrel2 ; destruct H0 ; eauto ; try congruence ; try (destruct H0 ; congruence).
+    * apply EundefMpz with u;[easy|].  inversion Hrel2; destruct H0; try congruence || (destruct H0 ; congruence) ;simpl in *.
+        + right. now exists (proj1_sig sub2 l).
+        + destruct H0. right. now  exists None.
     * now apply Enone.
 Qed.
 
+
+Fact trans_env_partial_order : transitive Ω (fun e e' => e ⊑ e')%env.
+Proof.
+    intros e e' e'' [f1 H1] [f2 H2]. exists (exist _ _ (bijective_comp_bijective f1 f2)).
+    now apply _trans_env_partial_order with e'. 
+Qed.
+
+
+(* 
 Fact antisym_env_partial_order : forall env env',
     env_partial_order env' env /\ env_partial_order env env' -> forall v, env v = env' v.
 
 Proof.
-    intros env env' [H1 H2] v. specialize (H1 v). inversion H1 ; try congruence.
+    intros env env' [[[f1 Hf1] H1] [[f2 Hf2] H2]] v. specialize (H1 v). inversion H1.
+    - congruence. 
+    - destruct H2 with v; try congruence. clear H1. clear H2. simpl in *.
+       admit.
+    - congruence.
     - destruct H0 ; destruct H0;  destruct H2 with v; congruence.
     - destruct H0 ; destruct H0;  destruct H2 with v; congruence.
     - destruct H2 with v; destruct H0 ; try congruence  || (destruct H3; destruct H0 ; congruence).
-Qed.
+Qed. *)
 
 
 
-#[global] Add Relation Ω env_partial_order
+#[global] Add Relation Ω (fun e e' => e ⊑ e')%env
     reflexivity proved by refl_env_partial_order
     transitivity proved by trans_env_partial_order as Renv.
 
 
-Fact refl_mem_partial_order : reflexive 𝓜 mems_partial_order.
+
+Fact _refl_mem_partial_order : reflexive 𝓜  (fun e e' => mem_partial_order e e' (exist _ _ id_bijective)).
 Proof.
-    intros mem l. trivial. 
+    easy.
 Qed.    
 
-Fact trans_mem_partial_order : transitive 𝓜 mems_partial_order.
+Corollary refl_mem_partial_order : reflexive 𝓜  (fun e e' => e ⊑ e')%mem.
 Proof.
-    intros mem mem' mem'' H1 H2 l. destruct (mem l) eqn:L.
-    - erewrite H2 ; eauto. 
-    - discriminate.
+    eexists. apply _refl_mem_partial_order.
+Qed.    
+
+
+Fact _trans_mem_partial_order : forall (x y z: 𝓜) f1 f2, 
+    mem_partial_order x y f1 ->
+    mem_partial_order y z f2 -> 
+    mem_partial_order x z (exist _ _ (bijective_comp_bijective f1 f2)).
+Proof.
+    intros mem mem' mem'' sub1 sub2 Hrel1 Hrel2 l i H. simpl in *.
+    specialize (Hrel1 l i). apply Hrel1 in H as HH.
+    specialize (Hrel2 (proj1_sig sub1 l) i). now apply Hrel2 in HH.
 Qed.
 
 
-Fact antisym_mem_partial_order : forall mem mem', 
+Corollary trans_mem_partial_order : transitive 𝓜 (fun e e' => e ⊑ e')%mem.
+Proof.
+    intros e e' e'' [f1 H1] [f2 H2]. exists (exist _ _ (bijective_comp_bijective f1 f2)). now apply _trans_mem_partial_order with e'.
+Qed.
+
+(* Fact antisym_mem_partial_order : forall mem mem', 
     mems_partial_order mem mem' /\ mems_partial_order mem' mem -> forall l, mem l = mem' l.
 Proof.
     intros mem mem' [H1 H2] l. destruct (mem l) eqn:Heqn.
@@ -199,38 +311,102 @@ Proof.
     - destruct (mem' l) eqn:Heqn'. apply H2 in Heqn'.
         + congruence.
         + easy.
-Qed.
+Qed. *)
 
 
-#[global] Add Relation 𝓜 mems_partial_order
+#[global] Add Relation 𝓜 (fun e e' => e ⊑ e')%mem
     reflexivity proved by refl_mem_partial_order 
     transitivity proved by trans_mem_partial_order as mem.
 
     
-Fact refl_env_mem_partial_order : forall ev, (ev ⊑ ev)%envmem.
+Fact _refl_env_mem_partial_order : reflexive Env (fun e e' => env_mem_partial_order e e' (exist _ _ id_bijective))%envmem.
 Proof.
-    intros. split.
-    - pose refl_env_partial_order as r. now unfold reflexive in r.
-    - pose refl_mem_partial_order as r. now unfold reflexive in r.
+    intros e.  split.
+    -  apply _refl_env_partial_order.
+    - apply _refl_mem_partial_order.
 Qed.
 
-Fact eq_env_partial_order :  forall e e' v z, (e ⊑ e')%env ->  
+
+Corollary refl_env_mem_partial_order : reflexive Env (fun e e' => e ⊑ e')%envmem.
+    eexists. apply _refl_env_mem_partial_order.
+Qed.
+
+
+Fact _trans_env_mem_partial_order : forall (x y z: Env) f1 f2, 
+    env_mem_partial_order x y f1 ->
+    env_mem_partial_order y z f2 -> 
+    env_mem_partial_order x z (exist _ _ (bijective_comp_bijective f1 f2)).
+Proof.
+    intros e e' e'' f1 f2 [Henv1 Hmem1] [Henv2 Hmem2]. split.
+    - now apply _trans_env_partial_order with e'.
+    - now eapply _trans_mem_partial_order.
+Qed.
+
+Fact trans_env_mem_partial_order : transitive Env (fun e e' => e ⊑ e')%envmem.
+Proof.
+        intros e e' e'' [f1 H1] [f2 H2].   exists (exist _ _ (bijective_comp_bijective f1 f2)).
+        now apply _trans_env_mem_partial_order with e'.
+Qed.
+
+
+#[global] Add Relation Env (fun e e' => e ⊑ e')%envmem  
+    reflexivity proved by refl_env_mem_partial_order 
+    transitivity proved by trans_env_mem_partial_order as env_mem.
+
+
+(* Fact eq_env_partial_order :  forall e e' v z, (e ⊑ e')%env ->  
     e v = Some (Def z) -> e' v = Some (Def z).
 Proof.
-    intros e e' v z Hrel He. destruct Hrel with v; congruence.
+    intros e e' v z Hrel He. destruct Hrel. specialize (H v). inversion H; try congruence. rewrite He in H0. injection H0 as H0. subst.
+    intros e e' v z Hrel He. destruct Hrel. specialize (H v). inversion H. try congruence.
+Qed. *)
+
+
+
+Fact empty_env_refl_any_sub: forall s, env_partial_order empty_env empty_env s.
+Proof.
+    intros s v. now constructor.  
 Qed.
 
+Fact empty_mem_refl_any_sub:  forall s, mem_partial_order empty_env empty_env s.
+Proof.
+    intros s v z H. inversion H. 
+Qed.
 
+Fact empty_env_mem_refl_any_sub:  forall s, env_mem_partial_order empty_env empty_env s.
+Proof.
+        intros s. split.
+        - apply empty_env_refl_any_sub.
+        - apply empty_mem_refl_any_sub.
+Qed.
 
 Fact eq_int_env_mem_partial_order :  forall e e' v n, (e ⊑ e')%envmem -> 
     e v = Some (Def (VInt n)) -> e' v = Some (Def (VInt n)).
 Proof.
-    intros e e' v z [He Hm] Hsome. destruct (He v); congruence.  
+    intros e e' v z [f [He Hm]] Hsome. destruct (He v); congruence.  
 Qed.
 
-Open Scope utils_scope.
 
-Fact sym_env_cond : forall (env env' : Ω), 
+
+Fact eq_mpz_env_mem_partial_order :  forall e e' sub, 
+    env_mem_partial_order e e' sub -> 
+    forall v mpz, e v = Some (Def (VMpz mpz)) -> e' v = Some (induced sub (VMpz mpz)).
+Proof.
+    intros e e' sub [He Hm] v l Hsome. destruct (He v); try congruence.
+    - rewrite Hsome in H. now inversion H.
+    - destruct l;  simpl ; rewrite Hsome in H; now inversion H.
+Qed.
+
+Fact eq_defined_mpz_mem_partial_order : forall e e' sub, 
+    env_mem_partial_order e e' sub -> 
+    forall (l:location) z, e.(mstate) l = Some (Defined z) -> e'.(mstate) (proj1_sig sub l) = Some (Defined z).
+Proof.
+    intros e e' sub [_ Hmem] l z H. specialize (Hmem l).  now destruct Hmem with z.
+Qed.
+
+
+
+(* Fact sym_env_cond : forall (env env' : Ω), 
 (forall v, (dom env - dom env') v ) -> (env ⊑ env')%env -> (env' ⊑ env)%env.
 
 Proof.
@@ -238,10 +414,10 @@ Proof.
     - now exists n. 
     - now exists (VMpz l).
     - destruct H1.
-        + now exists (UInt n). 
+        + now exists UInt. 
         + destruct H1. now exists x. 
     - destruct H1.
-        + now exists (UMpz n).
+        + now exists UMpz.
         + destruct H1 as [x]. now exists (VMpz x).
     - destruct Hin. destruct env. simpl in *. congruence.
 Qed.
@@ -250,81 +426,130 @@ Corollary sym_env_cond_mem : forall (ev ev' : Env),
 (forall v, (dom ev - dom ev') v ) -> (ev ⊑ ev')%envmem ->  (mkEnv ev' ev ⊑ mkEnv ev ev')%envmem.
 Proof.
     intros [env mem]. split. now apply sym_env_cond. now destruct H0.
-Qed.
+Qed. *)
 
 
-Corollary eq_env_partial_order_add :  forall (e e' :Ω) v v' z z',  (e ⊑ e')%env ->  
+(* Corollary eq_env_partial_order_add :  forall (e e' :Ω) v v' z z',  (e ⊑ e')%env ->  
     v <> v' ->
     e v = Some (Def z) -> (e'{v'\z'}) v = Some (Def z).
 Proof.
     intros [v l] [v' l'] var var' z z' Hrel Hneq H. 
     pose proof (eq_env_partial_order {|vars:=v;binds:=l|} {|vars:=v';binds:=l'|} var z Hrel H).
     pose proof (p_map_not_same {| vars := v'; binds := l' |} var var' z' Hneq). congruence.
-Qed.
+Qed. *)
 
 
-Fact eq_mem_partial_order :  
+(* Fact eq_mem_partial_order :  
     forall mem mem' z l, (mem ⊑ mem')%mem -> z <> None ->  
     mem l = z ->  mem' l = z.
 Proof.
     intros. destruct z.
     - edestruct H; eauto.
     - contradiction.
-Qed.
+Qed. *)
 
 
+Fact mem_def_partial_order_add : forall e e' sub, env_mem_partial_order e e' sub -> 
 
-Fact env_partial_order_add : forall Ω₀ Ω₀', (Ω₀ ⊑ Ω₀')%env -> 
-    (forall var' z, 
-    Ω₀ <| vars ::= fun x => x{var' \ z} |> ⊑  Ω₀' <| vars ::= fun x => x{var' \ z} |>
-    )%env.
-Proof with auto with rac_hint.
-    intros [v l][v' l'] H x z var. destruct (string_dec x var) as [Heq|Hneq].
-    - subst. simpl. specialize (H var). destruct z. 
-        + destruct v0.
-            * apply EsameInt with n ;  apply p_map_same.
-            * apply EsameMpz with l0; apply p_map_same.
-        + destruct uv.
-            ++ apply EundefInt with n ; simpl...
-            ++ apply EundefMpz with l0 ; simpl...
+    (forall (l:location) (z : mpz_val),
 
-    - apply not_eq_sym in Hneq. epose proof (p_map_not_same v var x ?[z] Hneq) as H0. simpl. remember (v var) as res. destruct res as [z'|].
-        * destruct z'.
-            + { 
-                destruct v0.
-                - apply EsameInt with n ; simpl.
-                    + apply H0.
-                    + apply p_map_not_same_eq in H0... epose proof (eq_env_partial_order_add  _ _ _ _ _ _ H). 
-                        now apply H1.
-                - apply EsameMpz with l0; simpl... epose proof (eq_env_partial_order_add  _ _ _ _ _ _ H).
-                    symmetry in Heqres. specialize (H1 Hneq Heqres). simpl in H1. apply H1.
-            }
+            env_mem_partial_order 
+                (e <| mstate ::={{l \ z}} |>) 
+                (e' <| mstate ::={{proj1_sig sub l \ z}} |>) sub
 
-            + {
-                destruct uv.
-                - eapply EundefInt ;subst ;simpl. 
-                    + apply H0.
-                    + destruct H with var ; pose proof (p_map_not_same_eq v' var x z) as Hres; simpl in *; try congruence.
-                        destruct H2.
-                        * specialize (Hres  (Some (Undef (UInt n))) Hneq). left. apply Hres. congruence.
-                        * destruct H2 as [x0]. specialize (Hres  (Some (Def (VInt x0))) Hneq). right. exists x0. now apply Hres.
-                - eapply EundefMpz ; subst ; simpl.
-                    + apply H0.
-                    + destruct H with var ; pose proof (p_map_not_same_eq v' var x z) as Hres; simpl in * ; try congruence.
-                        destruct H2.
-                        * specialize (Hres  (Some (Undef (UMpz l0))) Hneq). left.  apply Hres. congruence.
-                        * destruct H2 as [l0']. specialize (Hres  (Some (Def (VMpz l0'))) Hneq). right. exists l0'. now apply Hres.
-            }
-        * now apply Enone.
-Qed.
-
-Fact mems_partial_order_add : forall M₀ M₀', mems_partial_order M₀ M₀' -> 
-    (forall l mi, mems_partial_order ((M₀) {l \ mi}) ((M₀') {l \ mi})).
+    ).
 Proof.
-    intros mem mem' H l mi. intros l' i H1. destruct (eq_dec l' l).
-    - subst. pose proof (p_map_same mem l mi). rewrite H0 in H1. injection H1 as eq. subst.  apply p_map_same.
-    - pose proof (p_map_not_same mem l' l mi n). rewrite H0 in H1. apply p_map_not_same_eq ; auto.
+        intros e e' sub [Henv Hmem] l z. split; [trivial|].
+        intros l'.  intros mpz H. simpl in *. destruct (eq_dec l l').
+        - subst. unfold p_map_back in H. rewrite p_map_same in H. inversion H. subst.
+            unfold p_map_back. apply p_map_same.
+        - unfold p_map_back in H. rewrite p_map_not_same in H; [|auto]. apply p_map_not_same_eq.
+            * destruct sub. simpl in *. now rewrite <- bijective_eq_iff_f_eq. 
+            * specialize (Hmem l'). now apply Hmem in H. 
 Qed.
+
+
+Fact env_partial_order_add : forall Ω₀ Ω₀' sub, 
+    env_mem_partial_order Ω₀ Ω₀' sub -> 
+    (forall var' z, 
+    env_mem_partial_order (Ω₀ <| env; vars ::= {{var' \ z}} |>) (Ω₀' <| env ; vars ::= {{var' \ induced sub z}} |>) sub
+    )%envmem.
+Proof with eauto with rac_hint.
+    intros [v l][v' l'] sub H x z.  split.
+    - intros var. destruct (string_dec x var) as [Heq|Hneq].
+        -- subst. simpl. destruct z. 
+            + destruct v0.
+                * apply EsameInt with n ;  apply p_map_same.
+                * destruct l0 eqn:L0.
+                    ++ apply EsameMpz with l1; apply p_map_same.
+                    ++ apply ENullPtr; simpl; now apply p_map_same.
+            + destruct uv.
+                ++ apply EundefInt with u; autounfold with rac_hint; simpl...
+                ++ apply EundefMpz with u; autounfold with rac_hint; simpl...
+
+        -- apply not_eq_sym in Hneq. epose proof (p_map_not_same v var x ?[z] Hneq) as H0. simpl. remember (v var) as res. destruct res as [z'|] eqn:RES.
+            * destruct z' eqn:Z.
+                + { 
+                    destruct v0.
+                    - apply EsameInt with n ; simpl.
+                        + apply H0.
+                        + autounfold with rac_hint. apply p_map_not_same_eq...  apply (eq_int_env_mem_partial_order (mkEnv v l) (mkEnv v' l') var n)... now exists sub.
+                    - destruct l0.
+                        + apply EsameMpz with l0; simpl...
+                            autounfold with rac_hint. apply p_map_not_same_eq...
+                            now apply (eq_mpz_env_mem_partial_order  (mkEnv v l) (mkEnv v' l') sub H var (Some l0)).
+                        + apply ENullPtr... simpl.  apply p_map_not_same_eq...
+                         now apply (eq_mpz_env_mem_partial_order  (mkEnv v l) (mkEnv v' l') sub H var None).
+                }
+
+                + {
+                    destruct uv.
+                    - apply EundefInt with u;subst ;simpl. 
+                        + apply H0.
+                        + destruct H. specialize (H var). simpl in *. destruct H; try congruence. destruct H2 as [[n H2]|[n H2]].
+                            ++ left. exists n. now apply p_map_not_same_eq.
+                            ++ right. exists n. now apply p_map_not_same_eq.
+                    - apply EundefMpz with u; subst ; simpl.
+                        + apply H0.
+                        + destruct H. specialize (H var). simpl in *. destruct H; try congruence. destruct H2 as [[n H2]|[n H2]].
+                            ++ left. exists n. now apply p_map_not_same_eq.
+                            ++ right. exists n. now apply p_map_not_same_eq.
+                }
+            * now apply Enone.
+
+    - intros loc. intros mpz Hloc. simpl in *. destruct  H as [_ H]. specialize (H loc mpz). now destruct H. 
+Qed.
+
+
+
+
+
+Fact env_mem_partial_order_add_mem : forall e1 e1' e2 e2' sub, 
+    env_mem_partial_order e1 e2 sub  -> 
+    env_mem_partial_order e1' e2' sub -> 
+    env_mem_partial_order (e1 <| mstate := e1' |>) (e2 <| mstate := e2' |>) sub.
+    
+Proof with auto with rac_hint.
+    intros e1 e1' e2 e2' sub [H1e H1m] [H2e H2m]. now split.
+Qed.
+
+
+
+Fact same_int_any_sub :  forall e e' xargs zargs sub, 
+    List.length xargs = List.length zargs -> 
+    let vargs := List.map (fun x => Def (VInt x)) zargs in 
+    env_mem_partial_order e e' sub -> 
+    env_mem_partial_order 
+        (e <| env; vars ::= p_map_addall_back xargs vargs |>)
+        (e' <| env; vars ::= p_map_addall_back xargs vargs |>) sub.
+Proof.
+    intros e e' xargs. simpl. induction xargs; intros  zargs sub H Henv.
+    - simpl in H. symmetry in H. apply List.length_zero_iff_nil in H. subst. simpl.
+        unfold p_map_addall_back. unfold p_map_addall_front. simpl.   admit. (* should be able to use Henv *)
+    - simpl in *.  destruct zargs as [| zargs_hd zargs_tl] eqn:zargsEqn; [discriminate|].  
+        destruct (IHxargs zargs_tl sub) as [Hindenv _]; auto. clear IHxargs. simpl in *.
+        unfold p_map_addall_back. unfold p_map_addall_front. simpl. admit.
+Admitted.
 
 
 
@@ -338,7 +563,7 @@ Definition _no_env_mpz_aliasing (ev : Ω) : Prop :=
 
 
 Definition type_of_value : option 𝕍 -> option 𝔗 := fun v => match v with
-| Some (VInt _) | Some (UInt _)  => Some C_Int
+| Some (VInt _) | Some (UInt _) => Some C_Int
 | Some (VMpz _) | Some (UMpz _) => Some (T_Ext Mpz)
 | None => None
 end.
@@ -350,16 +575,21 @@ Proof.
 Qed.
 
 
-Fact env_same_ty : forall  (Ω Ω' : Ω) v t, (Ω ⊑ Ω')%env -> t <> None -> type_of_value (Ω v) = t -> type_of_value (Ω' v) = t.
+Fact induced_ty_same v (sub:σ) : type_of_value (Some (induced sub v)) = type_of_value (Some v).
 Proof.
-    intros. 
+    destruct v; simpl; [|trivial]. destruct v; simpl; [trivial|]. now destruct l. 
+Qed.
+
+Fact env_same_ty : forall  (Ω Ω' : Env) v t, (Ω ⊑ Ω')%envmem -> t <> None -> type_of_value (Ω v) = t -> type_of_value (Ω' v) = t.
+Proof.
+    (* intros. 
     match goal with | IncRel : (_ ⊑ _)%env |- _ =>  destruct IncRel with v ; subst end ;
     match goal with 
     | L : apply_env ?Ω v = _,  R : apply_env ?Ω' v = _  |- _ => now rewrite L,R 
     | L : apply_env ?Ω v = _,  R : apply_env ?Ω' v = _ \/ _ |- _ => destruct R as [SomeUInt | [ x Some_n ]]; [now rewrite L,SomeUInt | now rewrite L,Some_n] 
     | L : _ = None,  Contra : _ <> None |- _ =>  now rewrite L in Contra
-    end.
-Qed.
+    end. *)
+Admitted.
 
 
 
@@ -419,7 +649,7 @@ Definition Γ := Γᵥ ⨉ Γᵢ.
 (* See 5.1. (𝔏 ⇀ 𝐼) is the interval infered for each function arguments but how to make it decidable ? *)
 Axiom eq_dec_bindings : forall (e1 e2 : (𝔏 ⨉ (𝔏 ⇀ 𝐼))), {e1 = e2} + {e1 <> e2}. 
 
-#[global] Instance eqdec_bindings : EqDec (𝔏 ⨉ (𝔏 ⇀ 𝐼)) := {
+#[global] Instance eqdec_bindings : EqDecC (𝔏 ⨉ (𝔏 ⇀ 𝐼)) := {
     eq_dec := eq_dec_bindings
 }.
 
