Arithmetic/theories/Languages/MiniGMP/Lemmas.v
@@ -4,21 +4,46 @@ From RecordUpdate Require Import RecordUpdate.
 From Coq Require Import ZArith.ZArith.
 Open Scope Z_scope. 
 
+(* helper lemma for gmp cmp semantics *)
+Fact cmp_induced : forall zx zy (b: 𝕍) sub,
+    (zx > zy <-> b = one) /\ (zx < zy <-> b = sub_one) /\ (Z.eq zx zy <-> b = zero)
+    -> 
+    (zx > zy <-> induced sub b = one) /\
+(zx < zy <-> induced sub b = sub_one) /\ (Z.eq zx zy <-> induced sub b = zero).
+Proof.
+    intros zx zy b sub (Hone & Hsubone &Hzero). split.
+    - split.
+        * intros Hzxzy. apply Hone in Hzxzy. now subst.
+        * intros Hzxzy. apply induced_int_iff in Hzxzy. inversion Hzxzy. now apply Hone.
+    - split.
+       * split.
+            + intros Hzxzy. apply Hsubone in Hzxzy. now subst.
+            + intros Hzxzy. apply induced_int_iff in Hzxzy. inversion Hzxzy. now apply Hsubone.
+        * split.
+            + intros Hzxzy. apply Hzero in Hzxzy. now subst.
+            + intros Hzxzy. apply induced_int_iff in Hzxzy. inversion Hzxzy. now apply Hzero.
+Qed.
+
+
+
 Lemma _weakening_of_gmp_statements_semantics_1 : 
     _weakening_of_statement_semantics_1 Empty_exp_sem _gmp_stmt_sem
 .
-Proof with eauto using eq_env_partial_order, eq_mem_partial_order,refl_env_mem_partial_order with rac_hint ; try easy.
+Proof with eauto using refl_env_mem_partial_order with rac_hint ; try easy.
     intros Hweak f ev₀ s ev₁.
-    - intro Hderiv. induction Hderiv; intros ev₀' [Henv Hmem]; epose proof (fun y => weakening_of_c_expression_semantics y ev₀) as weak_exp.
+    - intro Hderiv. induction Hderiv; intros ev₀' sub Henvmem; 
+        epose proof (fun y => weakening_of_c_expression_semantics y ev₀) as weak_exp;
+        pose proof (eq_defined_mpz_mem_partial_order ev₀ ev₀' sub Henvmem) as eq_defined ;
+        pose proof (eq_mpz_env_mem_partial_order ev₀ ev₀' sub Henvmem) as  eq_mpz ;
+        pose proof (mem_def_partial_order_add) as mpz_add;
+        pose proof (env_partial_order_add ev₀ ev₀' sub Henvmem) as env_add.
         (* init *)
-        * exists (ev₀' <| env ; vars ::= {{x \ Def (VMpz (Some l))}} |> <| mstate ::= {{l \Defined 0}} |> ). split.
-            + split. 
-                ++ apply env_partial_order_add... 
-                ++ apply mems_partial_order_add...
-            + apply S_init.
-                ++ intros v Hcontra. 
+        * exists (ev₀' <| env ; vars ::= {{x \ Def (VMpz (Some (proj1_sig sub l)))}} |> <| mstate ::= {{proj1_sig sub l \Defined 0}} |> ). split.
+            + now apply mpz_add.
+            + apply S_init with u.
+                ++ intros v Hcontra.
                     (* the fact v is not bound to mpz location l by Ω₀ doesn't mean 
-                        that v will also not be bound to mpz location l by Ω₀' 
+                        that v will also not be bound to mpz location l' by Ω₀' 
                     *) 
                     admit.
                 ++ (* the semantic of ⊑ only ensures a defined mpz must stay the same, 
@@ -27,41 +52,43 @@ Proof with eauto using eq_env_partial_order, eq_mem_partial_order,refl_env_mem_p
                     *)
                     admit.
         (* clear *)
-        * exists (ev₀' <| env ; vars ::= {{x\Def (VMpz None)}} |><| mstate ::= {{a \ Undefined u}} |>). split.
-            + split.
-                ++ apply env_partial_order_add...
-                ++ apply mems_partial_order_add...
-            + constructor... 
+        * exists (ev₀' <| env ; vars ::= {{x\Def (VMpz None)}} |><| mstate ::= {{(proj1_sig sub) a \ Undefined u}} |>). split.
+            + now apply mpz_add.
+            + apply S_clear. now apply (eq_mpz x (Some a)).
 
         (* set_i *)
-        * exists (ev₀' <| mstate ::= {{a \ Defined (z) ̇}} |>). split.
-            + split... intro n. apply (mems_partial_order_add ev₀ ev₀' Hmem a z ̇).  
-            + apply S_set_i. eapply eq_env_partial_order... apply weak_exp...   
+        * exists (ev₀' <| mstate ::= {{(proj1_sig sub) a \ Defined (z) ̇}} |>).  split...
+            apply S_set_i...
+            ++ now apply (eq_mpz x (Some a)).
+            ++ apply weak_exp... now exists sub.
 
         (* set_z *)
-        * exists (ev₀' <| mstate ::= {{a \ z}} |>). split.
-            + split... intro n0.  apply (mems_partial_order_add ev₀ ev₀' Hmem a).
-            + apply S_set_z with n...
+        * exists (ev₀' <| mstate ::= {{(proj1_sig sub) a \Defined z}} |>). split...
+            + apply S_set_z with (proj1_sig sub n)...
+                ++ now apply (eq_mpz x (Some a)).
+                ++ now apply (eq_mpz y (Some n)).
 
         (* get_int *)
-        *  eexists (ev₀' <| env ; vars ::= fun e =>  e{x \ Def (VInt (zy ⁱⁿᵗ ir))} |>)...  split.
-            + split... simpl. pose proof env_partial_order_add...
-            + apply S_get_int with ly...
+        *  exists (ev₀' <| env ; vars ::= fun e =>  e{x \ Def (VInt (zy ⁱⁿᵗ ir))} |>). split...
+            apply S_get_int with (proj1_sig sub ly)... now apply (eq_mpz y (Some ly)).
         
         (* set_s *)
-        * exists (ev₀' <| mstate ::= {{lx \ Defined zx}} |>). split.
-            + split... apply (mems_partial_order_add ev₀ ev₀' Hmem lx zx). 
-            + constructor...
+        * exists (ev₀' <| mstate ::= {{(proj1_sig sub) lx \ Defined zx}} |>). split...
+            constructor... now apply (eq_mpz x (Some lx)).
 
         (* cmp *)
-        *  eexists (ev₀' <| env ; vars ::= fun e => e{c \ b} |>). split.
-            + split... simpl. pose env_partial_order_add...
-            + apply S_cmp with lx ly zx zy...        
-        
+        *  exists (ev₀' <| env ; vars ::= fun e => e{c \induced sub b} |>). 
+            split ... apply S_cmp with (proj1_sig sub lx) (proj1_sig sub ly) zx zy...
+                ++ now apply (eq_mpz x (Some lx)).
+                ++ now apply (eq_mpz y (Some ly)).
+                ++ now apply cmp_induced.
         (* op *)
-        * eexists (ev₀' <| mstate ::= {{lr \Defined (⋄ bop zx zy)}} |>). split.
-            + split... intro n. apply mems_partial_order_add...   
-            + apply S_op with lx ly ; try apply weak_exp...  
+        * eexists (ev₀' <| mstate ::= {{(proj1_sig sub) lr \Defined (⋄ bop zx zy)}} |>). split.
+            + now apply (mem_def_partial_order_add).
+            + apply S_op with (proj1_sig sub lx) (proj1_sig sub ly)...
+                ++ now apply (eq_mpz x (Some lx)).
+                ++ now apply (eq_mpz y (Some ly)).
+                ++ now apply (eq_mpz r (Some lr)).
 Admitted.
 
 Definition weakening_of_gmp_statements_semantics_1 := 
